Second attempt on multi level generalization.
Tried to prove some real functions' security. Started from cache (lowest) layer.

src/BasicSecurity2.v
@@ -16,6 +16,7 @@ Require Import ProofIrrelevance.
 Require Import BasicProg.
 Require Import Array.
 Require Import Bytes.
+Require Import Cache. 
 
 Set Implicit Arguments.
 
@@ -31,80 +32,83 @@ Qed.
 
 Hint Resolve sync_invariant_possible_sync.
 
+Definition pred_upd_w (pre: @pred addr addr_eq_dec _) (a: addr) (v: valu):=
+  fun m => forall (m': @Mem.mem addr addr_eq_dec _), 
+  exists vs, m' a = Some vs -> m = Mem.upd m' a (v, vsmerge vs) -> pre m' . 
 
-(* 
-    Meaning of the definition:
-      Take two memories 
-          m1 = x \union mp
-          m2 = y \union mp
-      Assume: 
-          F1 x
-          F2 y
-          pre mp
-          If p executes with m1 vm hm, then produces out1
-       Then:
-          there exists two memories such that
-              m1' = x' \union mr
-              m2' = y' \union mr
-          memories are m1'(m2') vm' hm' after executing p on m1(m2)
-          output of both executions is r
-          post mr
-        OR
-          "same for crash"
-*)
-(* Frames does not say for the remainder memory is unchanged or not. *)
-(* 
-    Can we say
-      Defintion pequal P Q := forall m, P m <-> Q m.
-      Lemma exists_diskIs: forall F, exists p m, F m -> pequal F ([[ P ]] * diskIs m).
-*)
+Definition prog_secure T (p : prog T) (pre : pred) (post : pred) :=
+  forall m1 m2 mp F1 F2 out1 vm hm,
 
-
-Definition prog_secure T (p : prog T) (pre : pred):=
-  forall m1 m2 F1 F2 out1 vm hm,
-
-  (F1 * pre)%pred m1 ->
-  (F2 * pre)%pred m2 ->
+  (F1 * diskIs mp)%pred m1 ->
+  (F2 * diskIs mp)%pred m2 ->
+  pre mp ->
   exec m1 vm hm p out1 ->
 
-  (exists r m1' m2' vm' hm' post,
+  (exists r m1' m2' vm' hm' mr,
    out1 = Finished m1' vm' hm' r /\
    exec m2 vm hm p (Finished m2' vm' hm' r) /\
-   (F1 * post)%pred m1' /\
-   (F2 * post)%pred m2') \/
+   (F1 * diskIs mr)%pred m1' /\
+   (F2 * diskIs mr)%pred m2' /\
+   post mr) \/
 
-  (exists m1' m2' hm' post,
+  (exists m1' m2' hm' mc,
    out1 = Crashed _ m1' hm' /\
    exec m2 vm hm p (Crashed _ m2' hm') /\
-   (F1 * post)%pred m1' /\
-   (F2 * post)%pred m2').
+   (F1 * diskIs mc)%pred m1' /\
+   (F2 * diskIs mc)%pred m2').
 
-Definition rep partA partB :=
-  (arrayN ptsto_subset 0 partA *
-   arrayN ptsto_subset (length partA) partB)%pred.
+Definition addr_is_in {AT AEQ V} (a: AT) (pre: pred):=
+  forall (m: @Mem.mem AT AEQ V), pre m -> indomain a m.
 
-Definition read_partA a :=
-  Read a.
-
-Definition write_partA a v :=
-  Write a v.
-
-Definition extracts_to V (m m': @Mem.mem addr addr_eq_dec V) (pre: pred):=
-  exists m'', m = mem_union m' m'' /\ pre m'.
-
-Definition addr_is_in V (a: addr) (pre: pred):=
-  forall (m m1: @Mem.mem addr addr_eq_dec V), extracts_to m m1 pre -> exists (Fa: pred), (Fa * a|->?)%pred m1.
-  
-Definition valu0 := bytes2valu  (natToWord (valubytes*8) 0).
-
-
-Theorem read_partA_secure:
-  forall a partA partB,
-  addr_is_in a (rep partA partB) ->
-  prog_secure (Read a) (rep partA partB).
+Theorem read_secure:
+  forall a pre,
+  addr_is_in a pre ->
+  prog_secure (Read a) pre pre.
 Proof.
-  unfold prog_secure, addr_is_in, extracts_to; intros.
+  unfold prog_secure, addr_is_in; intros.
+   
+  pose proof H0 as Hx.
+  unfold sep_star in Hx. 
+  rewrite sep_star_is in Hx. 
+  unfold sep_star_impl in Hx.
+  repeat deex.
+  edestruct H; intros; eauto.
   
+  
+  pose proof H1 as Hx.
+  unfold sep_star in Hx. 
+  rewrite sep_star_is in Hx. 
+  unfold sep_star_impl in Hx.
+  repeat deex.
+  inversion H8; inversion H12; subst.
+  
+  inv_exec.
+  - (* Finished *)
+     left.
+     repeat eexists.
+     + econstructor.
+         econstructor.
+         admit. (* Possible to prove from H2 H3 H4 H7 H11 H16 *)
+     + eauto.
+     + eauto.
+     + eauto.
+  - (* Failed *)
+    exfalso.
+    admit. (* Possible to prove from H4 H10 *)
+  - (* Crashed *)
+    right.
+    repeat eexists; eauto.
+  Unshelve.
+  constructor.
+Admitted.
+  
+Theorem write_secure:
+  forall a v pre,
+  addr_is_in a pre ->
+  prog_secure (Write a v) pre (pred_upd_w pre a v).
+Proof.
+  unfold prog_secure, addr_is_in, pred_upd_w; intros.
+
   pose proof H0 as Hx.
   unfold sep_star in Hx. 
   rewrite sep_star_is in Hx. 
@@ -117,28 +121,297 @@ Proof.
   rewrite sep_star_is in Hx. 
   unfold sep_star_impl in Hx.
   repeat deex.
-  edestruct H; intros; eauto.
+  inversion H8; inversion H12; subst.
   
-  unfold rep in *.
-  rewrite <- arrayN_app in *.
-  apply arrayN_app in H7.
-  apply arrayN_app in H11.
   inv_exec.
   - (* Finished *)
-    left.
-    destruct_lift H4. destruct_lift H8.
-    repeat eexists.
-    + econstructor.
-      econstructor.
-      admit. (* Possible to prove from H2 H3 H4 H7 H11 H16 *)
-    + eauto.
-    + eauto.
+     left.
+     repeat eexists.
+     + econstructor.
+         econstructor.
+         admit. (* Possible to prove from H2 H3 H4 H7 H11 H16 *)
+     + eapply diskIs_sep_star_upd. 2: eauto. eauto.
+     + eapply diskIs_sep_star_upd. 2: eauto. eauto.
+     + intros.
+         assert (A: m4 = m').
+         * apply functional_extensionality; intros.
+            destruct (addr_eq_dec a x1);
+            subst. rewrite H5; rewrite H3; eauto.
+            erewrite <- Mem.upd_ne.
+            rewrite H9.
+            apply Mem.upd_ne.
+            all: omega.
+         * subst; eauto.
   - (* Failed *)
     exfalso.
     admit. (* Possible to prove from H4 H10 *)
   - (* Crashed *)
     right.
     repeat eexists; eauto.
-  Unshelve.
-  all: repeat constructor; apply valu0.
 Admitted.
+
+Theorem ret_secure:
+  forall T (x : T),
+  prog_secure (Ret x) emp emp.
+Proof.
+  unfold prog_secure; intros.
+  inv_exec.
+  left.
+  do 6 eexists; intuition.
+  eauto.
+  eauto.
+  eauto.
+Qed.
+
+Theorem bind_secure:
+  forall T1 T2 (p1 : prog T1) (p2 : T1 -> prog T2) pre post1 post2,
+  prog_secure p1 pre post1 ->
+  (forall x, prog_secure (p2 x) post1 post2) ->
+  prog_secure (Bind p1 p2) pre post2.
+Proof.
+  unfold prog_secure; intros.
+  inv_exec.
+  - (* p1 Finished *)
+    specialize (H _ _ _ _ _ _ _ _ H1 H2 H3 H11).
+    intuition; repeat deex; try congruence.
+    inversion H4; subst.
+    specialize (H0 r _ _ _ _ _ _ _ _ H5 H6 H8 H14).
+    intuition; repeat deex.
+    + left.
+      do 6 eexists; intuition eauto.
+    + right.
+      do 4 eexists; intuition eauto.
+  - (* p1 Failed *)
+    specialize (H _ _ _ _ _ _ _ _ H1 H2 H3 H10).
+    intuition; repeat deex; try congruence.
+  - (* p1 Crashed *)
+    specialize (H _ _ _ _ _ _ _ _ H1 H2 H3 H10).
+    intuition; repeat deex; try congruence.
+    right.
+    inversion H4; subst.
+    do 4 eexists; intuition.
+    constructor.
+    eauto.
+    eauto.
+    eauto.
+Qed.
+
+Theorem frame_secure:
+  forall T (p : prog T) pre post F,
+  prog_secure p pre post ->
+  prog_secure p (F * pre)%pred (F * post)%pred.
+Proof.
+  unfold prog_secure; intros.
+  eapply diskIs_sep_star_split in H2; repeat deex; intuition.
+  rewrite H6 in H0.
+  rewrite H6 in H1.
+  apply sep_star_assoc in H0.
+  apply sep_star_assoc in H1.
+  specialize (H _ _ _ _ _ _ _ _ H0 H1 H2 H3).
+  intuition; repeat deex.
+  - left.
+    apply sep_star_assoc in H7.
+    apply sep_star_assoc in H8.
+    rewrite (diskIs_sep_star_combine _ _ H4 H10) in H7; destruct_lift H7.
+    rewrite (diskIs_sep_star_combine _ _ H4 H10) in H8; destruct_lift H8.
+    do 6 eexists; intuition eauto.
+  - right.
+    apply sep_star_assoc in H7.
+    apply sep_star_assoc in H9.
+    assert ((diskIs mc) mc) by congruence.
+    rewrite (diskIs_sep_star_combine _ _ H4 H5) in H7; destruct_lift H7.
+    rewrite (diskIs_sep_star_combine _ _ H4 H5) in H9; destruct_lift H9.
+    do 4 eexists; intuition eauto.
+Qed.
+
+Theorem pimpl_secure:
+  forall T (p : prog T) pre pre' post post',
+  pre' =p=> pre ->
+  post =p=> post' ->
+  prog_secure p pre post ->
+  prog_secure p pre' post'.
+Proof.
+  unfold prog_secure; intros.
+  apply H in H4.
+  specialize (H1 _ _ _ _ _ _ _ _ H2 H3 H4 H5).
+  intuition; repeat deex.
+  left.
+  do 6 eexists; intuition eauto.
+Qed.
+
+Lemma ret_secure_frame:
+  forall T (x : T) F,
+  prog_secure (Ret x) F F.
+Proof.
+  intros.
+  eapply pimpl_secure.
+  3: eapply frame_secure.
+  3: apply ret_secure.
+  all: cancel.
+Qed.
+
+Lemma alertmodified_secure_frame:
+  forall F,
+  prog_secure (AlertModified) F F.
+Proof.
+  unfold prog_secure; intros.
+  inv_exec.
+  left.
+  do 6 eexists; intuition.
+  eauto.
+  eauto.
+  eauto.
+Qed.
+
+Lemma ret_secure_frame_impl_l:
+  forall T (x : T) F F',
+  F =p=> F' ->
+  prog_secure (Ret x) F F'.
+Proof.
+  intros.
+  eapply pimpl_secure.
+  eauto.
+  2: apply ret_secure_frame.
+  eauto.
+Qed.
+
+Transparent BUFCACHE.read.
+
+Theorem cache_writeback_secure:
+  forall a cs m,
+  addr_is_in a (BUFCACHE.rep cs m) ->
+  prog_secure (BUFCACHE.writeback a cs) (BUFCACHE.rep cs m) 
+                                                                    (BUFCACHE.rep cs m \/ exists w, (pred_upd_w (BUFCACHE.rep cs m) a w)).
+Proof.
+   unfold BUFCACHE.writeback in *; simpl in *; intros.
+   destruct (MapUtils.AddrMap.Map.find a (CSMap cs)) eqn:D; simpl in *.
+   - destruct p; simpl in *.
+      destruct b; simpl in *.
+      + eapply bind_secure.
+          * apply write_secure; eauto.
+          * intros.
+             apply ret_secure_frame_impl_l; cancel.
+      + apply ret_secure_frame_impl_l; cancel.
+  - apply ret_secure_frame_impl_l; cancel.
+Qed.
+
+Theorem cache_evict_secure:
+  forall a cs m,
+  addr_is_in a (BUFCACHE.rep cs m) ->
+  prog_secure (BUFCACHE.evict a cs) (BUFCACHE.rep cs m) 
+                                                            (BUFCACHE.rep cs m \/ exists w, (pred_upd_w (BUFCACHE.rep cs m) a w)).
+Proof.
+  unfold BUFCACHE.evict in *; simpl in *; intros.
+  eapply bind_secure.
+  - apply cache_writeback_secure; eauto.
+  - intros.
+    destruct (MapUtils.AddrMap.Map.find a (CSMap x)) eqn:D; simpl in *.
+    apply ret_secure_frame.
+    apply ret_secure_frame.
+Qed.
+
+Theorem cache_maybe_evict_secure:
+  forall m cs,
+  prog_secure (BUFCACHE.maybe_evict cs) (BUFCACHE.rep cs m) 
+                                                                     (BUFCACHE.rep cs m \/ exists a w, (pred_upd_w (BUFCACHE.rep cs m) a w)).
+Proof.
+  unfold BUFCACHE.maybe_evict in *; simpl in *; intros.
+  destruct (lt_dec (CSCount cs) (CSMaxCount cs)); simpl.
+  - apply ret_secure_frame_impl_l; cancel.
+  -  destruct (MapUtils.AddrMap.Map.find 0 (CSMap cs)) eqn:D.
+      + eapply bind_secure.
+      
+          * assert (A: {| CSMap := CSMap cs;
+                                 CSMaxCount := CSMaxCount cs;
+                                 CSCount := CSCount cs;
+                                 CSEvict := CSEvict cs |} = cs).
+             destruct cs; simpl; eauto.
+             rewrite A; apply cache_evict_secure.
+             unfold addr_is_in; intros.
+             unfold indomain.
+             admit. (* XXX *)
+          * intros; apply ret_secure_frame_impl_l; cancel.
+      + destruct (MapUtils.AddrMap.Map.elements (CSMap cs)) eqn:D0.
+          * eapply ret_secure_frame_impl_l; cancel.
+          * destruct p; simpl in *.
+             eapply bind_secure.
+             ** eapply cache_evict_secure.
+                 unfold addr_is_in; intros.
+                 unfold indomain.
+                 admit. (* XXX *)
+            ** intros; apply ret_secure_frame_impl_l; cancel.
+Admitted.
+
+Theorem cache_read_secure:
+  forall a m cs,
+  addr_is_in a (BUFCACHE.rep cs m) ->
+  prog_secure (BUFCACHE.read a cs) (BUFCACHE.rep cs m) 
+                                                            (BUFCACHE.rep cs m \/ exists a w, (pred_upd_w (BUFCACHE.rep cs m) a w)).
+Proof.
+    unfold BUFCACHE.read in *; simpl in *; intros.
+    eapply bind_secure; [ apply cache_maybe_evict_secure |  intros ].
+    destruct (MapUtils.AddrMap.Map.find a (CSMap x)) eqn:D.
+    - destruct p; apply ret_secure_frame.
+    - eapply bind_secure; [ apply alertmodified_secure_frame| intros].
+      eapply bind_secure; [apply read_secure | intros; apply ret_secure_frame].
+      unfold addr_is_in; intros.
+      destruct H0.
+      eauto.
+      destruct_lift H0.
+      admit. (* XXX *)
+Admitted.
+    
+    destruct (lt_dec (CSCount cs) (CSMaxCount cs)); simpl.
+  - apply ret_secure_frame_impl_l; cancel.
+  -  destruct (MapUtils.AddrMap.Map.find 0 (CSMap cs)) eqn:D.
+      + eapply bind_secure.
+      
+          * assert (A: {| CSMap := CSMap cs;
+                                 CSMaxCount := CSMaxCount cs;
+                                 CSCount := CSCount cs;
+                                 CSEvict := CSEvict cs |} = cs).
+             destruct cs; simpl; eauto.
+             rewrite A; apply cache_evict_secure.
+             unfold addr_is_in; intros.
+             unfold indomain.
+             admit. (* XXX *)
+          * intros; apply ret_secure_frame_impl_l; cancel.
+      + destruct (MapUtils.AddrMap.Map.elements (CSMap cs)) eqn:D0.
+          * eapply ret_secure_frame_impl_l; cancel.
+          * destruct p; simpl in *.
+             eapply bind_secure.
+             ** eapply cache_evict_secure.
+                 unfold addr_is_in; intros.
+                 unfold indomain.
+                 admit. (* XXX *)
+            ** intros; apply ret_secure_frame_impl_l; cancel.
+Admitted.
+
+
+
+
+
+
+
+
+
+
+
+
+
+
+
+
+
+
+
+
+
+
+
+
+
+
+
+
+
